Add wf and interp proofs for LetBindReturn
After    | File Name                           | Before   || Change    | % Change
----------------------------------------------------------------------------------
0m17.96s | Total                               | 0m00.90s || +0m17.07s | +1896.66%
----------------------------------------------------------------------------------
0m17.97s | Experiments/NewPipeline/UnderLetsWf | 0m00.90s || +0m17.07s | +1896.66%

src/Experiments/NewPipeline/UnderLetsWf.v
@@ -5,14 +5,19 @@ Require Import Crypto.Experiments.NewPipeline.LanguageInversion.
 Require Import Crypto.Experiments.NewPipeline.LanguageWf.
 Require Import Crypto.Experiments.NewPipeline.UnderLets.
 Require Import Crypto.Util.Tactics.BreakMatch.
+Require Import Crypto.Util.Tactics.DestructHead.
 Require Import Crypto.Util.Tactics.SpecializeAllWays.
+Require Import Crypto.Util.Tactics.SpecializeBy.
+Require Import Crypto.Util.Option.
 Import ListNotations. Local Open Scope list_scope.
 
+Import EqNotations.
 Module Compilers.
   Import Language.Compilers.
   Import LanguageInversion.Compilers.
   Import LanguageWf.Compilers.
   Import UnderLets.Compilers.
+  Import ident.Notations.
   Import expr.Notations.
   Import invert_expr.
 
@@ -141,126 +146,314 @@ Module Compilers.
     Proof. apply Interp_SubstVarOrIdent, Hwf. Qed.
   End SubstVarLike.
 
-  (*
   Module UnderLets.
-    Section with_var.
+    Import UnderLets.Compilers.UnderLets.
+    Section with_ident.
       Context {base_type : Type}.
-      Local Notation type := (type base_type).
-      Context {ident : type -> Type}
-              {var : type -> Type}.
-      Local Notation expr := (@expr base_type ident var).
+      Local Notation type := (type.type base_type).
+      Context {ident : type -> Type}.
+      Local Notation expr := (@expr.expr base_type ident).
+      Local Notation UnderLets := (@UnderLets base_type ident).
 
-      Inductive UnderLets {T : Type} :=
-      | Base (v : T)
-      | UnderLet {A} (x : expr A) (f : var A -> UnderLets).
+      Section with_var.
+        Context {var1 var2 : type -> Type}.
 
-      Fixpoint splice {A B} (x : @UnderLets A) (e : A -> @UnderLets B) : @UnderLets B
-        := match x with
-           | Base v => e v
-           | UnderLet A x f => UnderLet x (fun v => @splice _ _ (f v) e)
-           end.
+        Inductive wf {T1 T2} {P : list { t : type & var1 t * var2 t }%type -> T1 -> T2 -> Prop}
+          : list { t : type & var1 t * var2 t }%type -> @UnderLets var1 T1 -> @UnderLets var2 T2 -> Prop :=
+        | Wf_Base G e1 e2 : P G e1 e2 -> wf G (Base e1) (Base e2)
+        | Wf_UnderLet G A x1 x2 f1 f2
+          : expr.wf G x1 x2
+            -> (forall v1 v2, wf (existT _ A (v1, v2) :: G) (f1 v1) (f2 v2))
+            -> wf G (UnderLet x1 f1) (UnderLet x2 f2).
+        Global Arguments wf {T1 T2} P _ _ _.
 
-      Fixpoint splice_list {A B} (ls : list (@UnderLets A)) (e : list A -> @UnderLets B) : @UnderLets B
-        := match ls with
-           | nil => e nil
-           | cons x xs
-             => splice x (fun x => @splice_list A B xs (fun xs => e (cons x xs)))
-           end.
-
-      Fixpoint to_expr {t} (x : @UnderLets (expr t)) : expr t
-        := match x with
-           | Base v => v
-           | UnderLet A x f
-             => expr.LetIn x (fun v => @to_expr _ (f v))
-           end.
-      Fixpoint of_expr {t} (x : expr t) : @UnderLets (expr t)
-        := match x in expr.expr t return @UnderLets (expr t) with
-           | expr.LetIn A B x f
-             => UnderLet x (fun v => @of_expr B (f v))
-           | e => Base e
-           end.
-    End with_var.
-    Module Export Notations.
-      Global Arguments UnderLets : clear implicits.
-      Delimit Scope under_lets_scope with under_lets.
-      Bind Scope under_lets_scope with UnderLets.UnderLets.
-      Notation "x <-- y ; f" := (UnderLets.splice y (fun x => f%under_lets)) : under_lets_scope.
-      Notation "x <---- y ; f" := (UnderLets.splice_list y (fun x => f%under_lets)) : under_lets_scope.
-    End Notations.
+        Lemma wf_to_expr {t} (x : @UnderLets var1 (@expr var1 t)) (y : @UnderLets var2 (@expr var2 t))
+              G
+          : wf (fun G => expr.wf G) G x y -> expr.wf G (to_expr x) (to_expr y).
+        Proof.
+          intro Hwf; induction Hwf; cbn [to_expr]; [ assumption | constructor; auto ].
+        Qed.
+      End with_var.
+    End with_ident.
 
     Section reify.
-      Context {var : type.type base.type -> Type}.
       Local Notation type := (type.type base.type).
-      Local Notation expr := (@expr.expr base.type ident var).
-      Local Notation UnderLets := (@UnderLets.UnderLets base.type ident var).
-      Let type_base (t : base.type) : type := type.base t.
-      Coercion type_base : base.type >-> type.
+      Local Notation expr := (@expr.expr base.type ident).
+      Local Notation UnderLets := (@UnderLets.UnderLets base.type ident).
 
-      Let default_reify_and_let_binds_base_cps {t : base.type} : expr t -> forall T, (expr t -> UnderLets T) -> UnderLets T
-        := fun e T k
-           => match invert_expr.invert_Var e with
-              | Some v => k ($v)%expr
-              | None => if SubstVarLike.is_var_fst_snd_pair_opp e
-                        then k e
-                        else UnderLets.UnderLet e (fun v => k ($v)%expr)
-              end.
+      Section with_var.
+        Context {var1 var2 : type -> Type}.
+        Local Notation expr1 := (@expr.expr base.type ident var1).
+        Local Notation expr2 := (@expr.expr base.type ident var2).
+        Local Notation UnderLets1 := (@UnderLets.UnderLets base.type ident var1).
+        Local Notation UnderLets2 := (@UnderLets.UnderLets base.type ident var2).
 
-      Fixpoint reify_and_let_binds_base_cps {t : base.type} : expr t -> forall T, (expr t -> UnderLets T) -> UnderLets T
-        := match t return expr t -> forall T, (expr t -> UnderLets T) -> UnderLets T with
-           | base.type.type_base t
-             => fun e T k
-                => match invert_Literal e with
-                   | Some v => k (expr.Ident (ident.Literal v))
-                   | None => @default_reify_and_let_binds_base_cps _ e T k
-                   end
-           | base.type.prod A B
-             => fun e T k
-                => match invert_pair e with
-                   | Some (a, b)
-                     => @reify_and_let_binds_base_cps
-                          A a _
-                          (fun ae
-                           => @reify_and_let_binds_base_cps
-                                B b _
-                                (fun be
-                                 => k (ae, be)%expr))
-                   | None => @default_reify_and_let_binds_base_cps _ e T k
-                   end
-           | base.type.list A
-             => fun e T k
-                => match reflect_list e with
-                   | Some ls
-                     => list_rect
-                          _
-                          (fun k => k []%expr)
-                          (fun x _ rec k
-                           => @reify_and_let_binds_base_cps
-                                A x _
-                                (fun xe
-                                 => rec (fun xse => k (xe :: xse)%expr)))
-                          ls
-                          k
-                   | None => @default_reify_and_let_binds_base_cps _ e T k
-                   end
-           end%under_lets.
+        Local Ltac wf_reify_and_let_binds_base_cps_t Hk :=
+          repeat first [ lazymatch goal with
+                         | [ H : expr.wf _ ?e1 ?e2, H' : reflect_list ?e1 = Some _, H'' : reflect_list ?e2 = None |- _ ]
+                           => apply expr.wf_reflect_list in H; rewrite H', H'' in H; exfalso; clear -H; intuition congruence
+                         | [ H : expr.wf _ ?e1 ?e2, H' : reflect_list ?e2 = Some _, H'' : reflect_list ?e1 = None |- _ ]
+                           => apply expr.wf_reflect_list in H; rewrite H', H'' in H; exfalso; clear -H; intuition congruence
+                         | [ H : expr.wf _ (reify_list _) (reify_list _) |- _ ] => apply expr.wf_reify_list in H
+                         end
+                       | progress subst
+                       | progress destruct_head' False
+                       | progress expr.inversion_wf_constr
+                       | progress expr.inversion_expr
+                       | progress expr.invert_subst
+                       | progress destruct_head'_sig
+                       | progress destruct_head'_ex
+                       | progress destruct_head'_and
+                       | progress type.inversion_type
+                       | progress base.type.inversion_type
+                       | progress cbn [invert_Var invert_Literal ident.invert_Literal eq_rect f_equal f_equal2 type.decode fst snd projT1 projT2 invert_pair Option.bind combine list_rect length] in *
+                       | progress cbv [type.try_transport type.try_transport_cps CPSNotations.cps_option_bind CPSNotations.cpsreturn CPSNotations.cpsbind CPSNotations.cpscall type.try_make_transport_cps id] in *
+                       | rewrite base.try_make_transport_cps_correct in *
+                       | progress type_beq_to_eq
+                       | discriminate
+                       | congruence
+                       | apply Hk
+                       | exists nil; reflexivity
+                       | eexists (cons _ nil); reflexivity
+                       | rewrite app_assoc; eexists; reflexivity
+                       | progress wf_safe_t
+                       | match goal with
+                         | [ H : _ = _ :> ident _ |- _ ] => inversion H; clear H
+                         end
+                       | progress inversion_option
+                       | progress break_innermost_match_hyps
+                       | progress expr.inversion_wf_one_constr
+                       | progress expr.invert_match_step
+                       | match goal with |- wf _ _ _ _ => constructor end
+                       | match goal with
+                         | [ H : context[wf _ _ _ _] |- wf _ _ _ _ ] => apply H; eauto with nocore
+                         end
+                       | progress wf_unsafe_t_step
+                       | match goal with
+                         | [ H : context[match Compilers.reify_list ?ls with _ => _ end] |- _ ]
+                           => is_var ls; destruct ls; rewrite ?expr.reify_list_cons, ?expr.reify_list_nil in H
+                         | [ H : SubstVarLike.is_recursively_var_or_ident _ _ = _ |- _ ] => clear H
+                         | [ H : forall x y, @?A x y \/ @?B x y -> @?C x y |- _ ]
+                           => pose proof (fun x y pf => H x y (or_introl pf));
+                              pose proof (fun x y pf => H x y (or_intror pf));
+                              clear H
+                         end ].
 
-      Fixpoint let_bind_return {t} : expr t -> expr t
-        := match t return expr t -> expr t with
-           | type.base t
-             => fun e => to_expr (v <-- of_expr e; reify_and_let_binds_base_cps v _ Base)
-           | type.arrow s d
-             => fun e
-                => expr.Abs (fun v => @let_bind_return
-                                        d
-                                        match invert_Abs e with
-                                        | Some f => f v
-                                        | None => e @ $v
-                                        end%expr)
-           end.
+        Lemma wf_reify_and_let_binds_base_cps {t : base.type} {T1 T2} (e1 : expr1 (type.base t)) (e2 : expr2 (type.base t))
+              (k1 : expr1 (type.base t) -> UnderLets1 T1) (k2 : expr2 (type.base t) -> UnderLets2 T2)
+              (P : _ -> _ -> _ -> Prop) G
+              (Hwf : expr.wf G e1 e2)
+              (Hk : forall G' e1 e2, (exists seg, G' = seg ++ G) -> expr.wf G' e1 e2 -> wf P G' (k1 e1) (k2 e2))
+          : wf P G (reify_and_let_binds_base_cps e1 T1 k1) (reify_and_let_binds_base_cps e2 T2 k2).
+        Proof.
+          revert dependent G; induction t; cbn [reify_and_let_binds_base_cps]; intros;
+            try (cbv [SubstVarLike.is_var_fst_snd_pair_opp] in *; erewrite !SubstVarLike.wfT_is_recursively_var_or_ident by eassumption);
+            break_innermost_match; wf_reify_and_let_binds_base_cps_t Hk.
+          all: repeat match goal with H : list (sigT _) |- _ => revert dependent H end.
+          all: revert dependent k1; revert dependent k2.
+          all: lazymatch goal with
+               | [ H : length ?l1 = length ?l2 |- _ ]
+                 => is_var l1; is_var l2; revert dependent l2; induction l1; intro l2; destruct l2; intros
+               end;
+            wf_reify_and_let_binds_base_cps_t Hk.
+        Qed.
+
+        Lemma wf_let_bind_return {t} (e1 : expr1 t) (e2 : expr2 t)
+              G
+              (Hwf : expr.wf G e1 e2)
+          : expr.wf G (let_bind_return e1) (let_bind_return e2).
+        Proof.
+          revert dependent G; induction t; intros; cbn [let_bind_return]; cbv [invert_Abs];
+            wf_safe_t;
+            expr.invert_match; expr.inversion_wf; try solve [ wf_t ].
+          { apply wf_to_expr.
+            pose (P := fun t => { e1e2 : expr1 t * expr2 t | expr.wf G (fst e1e2) (snd e1e2) }).
+            pose ((exist _ (e1, e2) Hwf) : P _) as pkg.
+            change e1 with (fst (proj1_sig pkg)).
+            change e2 with (snd (proj1_sig pkg)).
+            clearbody pkg; clear Hwf e1 e2.
+            type.generalize_one_eq_var pkg; subst P; destruct pkg as [ [e1 e2] Hwf ].
+            cbn [fst snd proj1_sig proj2_sig] in *.
+            repeat match goal with
+                   | [ |- context[proj1_sig (rew [fun t => @sig (@?A t) (@?P t)] ?pf in exist ?P0 ?x ?p)] ]
+                     => progress replace (proj1_sig (rew pf in exist P0 x p)) with (rew [A] pf in x) by (case pf; reflexivity)
+                   | [ |- context[fst (rew [fun t => @prod (@?A t) (@?B t)] ?pf in pair ?x ?y)] ]
+                     => progress replace (fst (rew pf in pair x y)) with (rew [A] pf in x) by (case pf; reflexivity)
+                   | [ |- context[snd (rew [fun t => @prod (@?A t) (@?B t)] ?pf in pair ?x ?y)] ]
+                     => progress replace (fst (rew pf in pair x y)) with (rew [B] pf in y) by (case pf; reflexivity)
+                   end.
+            assert (H' : t = match t' with type.base t' => t' | _ => t end) by (subst; reflexivity).
+            revert pf.
+            rewrite H'; clear H'.
+            induction Hwf; break_innermost_match; break_innermost_match_hyps;
+              repeat first [ progress intros
+                           | progress type.inversion_type
+                           | progress base.type.inversion_type
+                           | progress wf_safe_t
+                           | progress cbn [of_expr fst snd splice eq_rect type.decode f_equal] in *
+                           | match goal with
+                             | [ H : forall pf : ?x = ?x, _ |- _ ] => specialize (H eq_refl)
+                             | [ H : forall x y (pf : ?a = ?a), _ |- _ ] => specialize (fun x y => H x y eq_refl)
+                             | [ |- wf _ _ _ _ ] => constructor
+                             end
+                           | solve [ eauto ]
+                           | apply wf_reify_and_let_binds_base_cps ]. }
+        Qed.
+      End with_var.
+
+      Lemma Wf_LetBindReturn {t} (e : expr.Expr t) (Hwf : expr.Wf e) : expr.Wf (LetBindReturn e).
+      Proof. intros ??; apply wf_let_bind_return, Hwf. Qed.
+
+      Local Ltac interp_to_expr_reify_and_let_binds_base_cps_t Hk :=
+        repeat first [ progress subst
+                     | progress destruct_head' False
+                     | progress destruct_head'_and
+                     | progress destruct_head' iff
+                     | progress specialize_by_assumption
+                     | progress expr.inversion_wf_constr
+                     | progress expr.inversion_expr
+                     | progress expr.invert_subst
+                     | progress destruct_head'_sig
+                     | progress destruct_head'_ex
+                     | progress destruct_head'_and
+                     | progress type.inversion_type
+                     | progress base.type.inversion_type
+                     | progress cbn [invert_Var invert_Literal ident.invert_Literal eq_rect f_equal f_equal2 type.decode fst snd projT1 projT2 invert_pair Option.bind to_expr expr.interp ident.interp ident.gen_interp type.eqv length list_rect combine In] in *
+                     | progress cbv [type.try_transport type.try_transport_cps CPSNotations.cps_option_bind CPSNotations.cpsreturn CPSNotations.cpsbind CPSNotations.cpscall type.try_make_transport_cps id] in *
+                     | rewrite base.try_make_transport_cps_correct in *
+                     | progress type_beq_to_eq
+                     | discriminate
+                     | congruence
+                     | apply Hk
+                     | exists nil; reflexivity
+                     | eexists (cons _ nil); reflexivity
+                     | rewrite app_assoc; eexists; reflexivity
+                     | rewrite expr.reify_list_cons
+                     | rewrite expr.reify_list_nil
+                     | progress interp_safe_t
+                     | match goal with
+                       | [ H : _ = _ :> ident _ |- _ ] => inversion H; clear H
+                       | [ H : forall t v1 v2, In _ _ -> _ == _, H' : In _ _ |- _ ] => apply H in H'
+                       end
+                     | progress inversion_option
+                     | progress break_innermost_match_hyps
+                     | progress expr.inversion_wf_one_constr
+                     | progress expr.invert_match_step
+                     | match goal with
+                       | [ |- ?R (expr.interp _ ?e1) (expr.interp _ ?e2) ]
+                         => solve [ eapply (@expr.wf_interp_Proper _ _ e1 e2); eauto ]
+                       | [ H : context[reflect_list (reify_list _)] |- _ ] => rewrite expr.reflect_reify_list in H
+                       | [ H : forall x y, @?A x y \/ @?B x y -> @?C x y |- _ ]
+                         => pose proof (fun x y pf => H x y (or_introl pf));
+                            pose proof (fun x y pf => H x y (or_intror pf));
+                            clear H
+                       end
+                     | progress interp_unsafe_t_step
+                     | match goal with
+                       | [ H : expr.wf _ (reify_list _) ?e |- _ ]
+                         => is_var e; destruct (reflect_list e) eqn:?; expr.invert_subst;
+                            [ rewrite expr.wf_reify_list in H | apply expr.wf_reflect_list in H ]
+                       | [ H : SubstVarLike.is_recursively_var_or_ident _ _ = _ |- _ ] => clear H
+                       | [ H : context[expr.interp _ _ = _] |- expr.interp _ (to_expr _) = ?k2 _ ]
+                         => erewrite H; clear H;
+                            [ match goal with
+                              | [ |- ?k (expr.interp ?ii ?e) = ?k' ?v ]
+                                => has_evar e;
+                                   let p := fresh in
+                                   set (p := expr.interp ii e);
+                                   match v with
+                                   | context G[expr.interp ii ?e']
+                                     => unify e e'; let v' := context G[p] in change (k p = k' v')
+                                   end;
+                                   clearbody p; reflexivity
+                              end
+                            | .. ]
+                       end ].
+
+      Lemma interp_to_expr_reify_and_let_binds_base_cps {t : base.type} {t' : base.type} (e1 : expr (type.base t)) (e2 : expr (type.base t))
+            G
+            (HG : forall t v1 v2, List.In (existT _ t (v1, v2)) G -> v1 == v2)
+            (Hwf : expr.wf G e1 e2)
+            (k1 : expr (type.base t) -> UnderLets _ (expr (type.base t')))
+            (k2 : base.interp t -> base.interp t')
+            (Hk : forall e1 v, defaults.interp e1 == v -> defaults.interp (to_expr (k1 e1)) == k2 v)
+        : defaults.interp (to_expr (reify_and_let_binds_base_cps e1 _ k1)) == k2 (defaults.interp e2).
+      Proof.
+        revert dependent G; revert dependent t'; induction t; cbn [reify_and_let_binds_base_cps]; intros;
+            try (cbv [SubstVarLike.is_var_fst_snd_pair_opp] in *; erewrite !SubstVarLike.wfT_is_recursively_var_or_ident by eassumption);
+            break_innermost_match; interp_to_expr_reify_and_let_binds_base_cps_t Hk.
+        all: repeat match goal with H : list (sigT _) |- _ => revert dependent H end.
+        all: revert dependent k1; revert dependent k2.
+        all: lazymatch goal with
+             | [ H : length ?l1 = length ?l2 |- _ ]
+               => is_var l1; is_var l2; revert dependent l2; induction l1; intro l2; destruct l2; intros
+             end;
+          interp_to_expr_reify_and_let_binds_base_cps_t Hk.
+      Qed.
+
+      Lemma interp_let_bind_return {t} (e1 e2 : expr t)
+            G
+            (HG : forall t v1 v2, List.In (existT _ t (v1, v2)) G -> v1 == v2)
+            (Hwf : expr.wf G e1 e2)
+        : defaults.interp (let_bind_return e1) == defaults.interp e2.
+      Proof.
+        revert dependent G; induction t; intros; cbn [let_bind_return type.eqv expr.interp] in *; cbv [invert_Abs respectful] in *;
+          repeat first [ progress wf_safe_t
+                       | progress expr.invert_subst
+                       | progress expr.invert_match
+                       | progress expr.inversion_wf
+                       | progress break_innermost_match_hyps
+                       | progress destruct_head' False
+                       | solve [ wf_t ]
+                       | match goal with
+                         | [ H : _ |- expr.interp _ (let_bind_return ?e0) == expr.interp _ ?e ?v ]
+                           => eapply (H e0 (e @ $v)%expr (cons _ _)); [ .. | solve [ wf_t ] ]; solve [ wf_t ]
+                         | [ H : _ |- expr.interp _ (let_bind_return ?e0) == expr.interp _ ?e ?v ]
+                           => cbn [expr.interp]; eapply H; [ | solve [ wf_t ] ]; solve [ wf_t ]
+                         end ];
+          [].
+        { pose (P := fun t => { e1e2 : expr t * expr t | expr.wf G (fst e1e2) (snd e1e2) }).
+          pose ((exist _ (e1, e2) Hwf) : P _) as pkg.
+          change e1 with (fst (proj1_sig pkg)).
+          change e2 with (snd (proj1_sig pkg)).
+          clearbody pkg; clear Hwf e1 e2.
+          type.generalize_one_eq_var pkg; subst P; destruct pkg as [ [e1 e2] Hwf ].
+          cbn [fst snd proj1_sig proj2_sig] in *.
+          repeat match goal with
+                 | [ |- context[proj1_sig (rew [fun t => @sig (@?A t) (@?P t)] ?pf in exist ?P0 ?x ?p)] ]
+                   => progress replace (proj1_sig (rew pf in exist P0 x p)) with (rew [A] pf in x) by (case pf; reflexivity)
+                 | [ |- context[fst (rew [fun t => @prod (@?A t) (@?B t)] ?pf in pair ?x ?y)] ]
+                   => progress replace (fst (rew pf in pair x y)) with (rew [A] pf in x) by (case pf; reflexivity)
+                 | [ |- context[snd (rew [fun t => @prod (@?A t) (@?B t)] ?pf in pair ?x ?y)] ]
+                   => progress replace (fst (rew pf in pair x y)) with (rew [B] pf in y) by (case pf; reflexivity)
+                 end.
+          assert (H' : t = match t' with type.base t' => t' | _ => t end) by (subst; reflexivity).
+          revert pf.
+          rewrite H'; clear H'.
+          induction Hwf; break_innermost_match; break_innermost_match_hyps;
+            repeat first [ progress intros
+                         | progress type.inversion_type
+                         | progress base.type.inversion_type
+                         | progress wf_safe_t
+                         | progress cbn [of_expr fst snd splice eq_rect type.decode f_equal to_expr] in *
+                         | match goal with
+                           | [ H : forall pf : ?x = ?x, _ |- _ ] => specialize (H eq_refl)
+                           | [ H : forall x (pf : ?a = ?a), _ |- _ ] => specialize (fun x => H x eq_refl)
+                           | [ H : forall x y (pf : ?a = ?a), _ |- _ ] => specialize (fun x y => H x y eq_refl)
+                           | [ H : forall x y z (pf : ?a = ?a), _ |- _ ] => specialize (fun x y z => H x y z eq_refl)
+                           | [ |- context[(expr_let x := _ in _)%expr] ] => progress cbn [expr.interp]; cbv [LetIn.Let_In]
+                           | [ H : context[expr.interp _ _ = expr.interp _ _] |- expr.interp _ _ = expr.interp _ _ ]
+                             => eapply H; eauto with nocore
+                           end
+                         | solve [ eauto ]
+                         | solve [ eapply expr.wf_interp_Proper; eauto ] ].
+          all: eapply interp_to_expr_reify_and_let_binds_base_cps with (k1:=Base) (k2:=(fun x => x)); eauto; wf_safe_t. }
+      Qed.
+
+      Lemma Interp_LetBindReturn {t} (e : expr.Expr t) (Hwf : expr.Wf e) : defaults.Interp (LetBindReturn e) == defaults.Interp e.
+      Proof.
+        apply interp_let_bind_return with (G:=nil); cbn [List.In]; eauto; tauto.
+      Qed.
     End reify.
-    Definition LetBindReturn {t} (e : expr.Expr t) : expr.Expr t
-      := fun var => let_bind_return (e _).
   End UnderLets.
-  Export UnderLets.Notations.
-   *)
 End Compilers.
